wip

cedar-lean/Cedar/Thm/Validation/Levels/WellFormed.lean
@@ -1194,6 +1194,13 @@ def AttributeRelation {α β : Type} (r : (Attr × α) → (Attr × β) → Prop
 def SameAttrs {α β : Type} (lhs : List (Attr × α)) (rhs : List (Attr × β)) :=
   lhs.map Prod.fst = rhs.map Prod.fst
 
+theorem SameAttrs_com {α β : Type} {lhs : List (Attr × α)} {rhs : List (Attr × β)}
+  (h : SameAttrs lhs rhs) :
+  SameAttrs rhs lhs
+  := by
+  simp [SameAttrs] at *
+  simp [h]
+
 
 def EvaluatesToOk (request : Request) (entities : Entities) (lhs : (Attr × Expr)) (rhs : Attr × Value) : Prop :=
   lhs.fst = rhs.fst ∧ evaluate lhs.snd request entities = .ok rhs.snd
@@ -1202,6 +1209,13 @@ theorem evalutesToOk_is_AttributeRelation (request : Request) (entities : Entiti
   AttributeRelation (EvaluatesToOk request entities)
   := by
   simp [AttributeRelation, EvaluatesToOk]
+  intros
+  simp only [*]
+
+theorem attrExprHasAttrType_is_AttributeRelation (c : Capabilities) (env : Environment) (l : Level) :
+  AttributeRelation (AttrExprHasAttrType c env l)
+  := by
+  simp [AttributeRelation, AttrExprHasAttrType]
   intros
   simp only [*]
 
@@ -1291,10 +1305,10 @@ theorem record_evaluation (attrs : List (Attr × Expr)) (map : Map Attr Value) {
   assumption
 
 
-theorem record_typing (attrs : List (Attr × Expr)) (ty : CedarType) {env : Environment} {c₁ c₂ : Capabilities} {l : Level}
-  (h₁ : typeOf (.record attrs) c₁ env (l == .infinite) = .ok (ty, c₂)) :
+theorem record_typing (attrs : List (Attr × Expr)) (ty_map : Map Attr QualifiedType) {env : Environment} {c₁ c₂ : Capabilities} {l : Level}
+  (h₁ : typeOf (.record attrs) c₁ env (l == .infinite) = .ok (.record ty_map, c₂)) :
   ∃ (tys : List (Attr × QualifiedType)),
-    List.Forall₂ (AttrExprHasAttrType c₁ env l) attrs tys ∧ SameAttrs attrs tys
+    List.Forall₂ (AttrExprHasAttrType c₁ env l) attrs tys ∧ SameAttrs attrs tys ∧ ty_map = Map.make tys
   := by
   simp [typeOf, List.mapM₂, List.attach₂] at h₁
   simp [List.mapM_pmap_subtype (λ (pair : (Attr × Expr)) => requiredAttr pair.fst (typeOf pair.snd c₁ env (l == .infinite)))] at h₁
@@ -1302,6 +1316,7 @@ theorem record_typing (attrs : List (Attr × Expr)) (ty : CedarType) {env : Envi
     <;> simp [well_typed, ok] at h₁
   rename_i tys
   exists tys
+  simp [h₁]
   apply attr_list_walk attrs tys (λ pair => requiredAttr pair.fst (typeOf pair.snd c₁ env (l == .infinite))) (AttrExprHasAttrType c₁ env l)
   apply well_typed
   simp [AttrBind]
@@ -1441,7 +1456,7 @@ theorem map_find_other_key {α β : Type}
   (h₃ : SameAttrs kvs₁ kvs₂)
   (h₄ : (Map.mk kvs₁).find? k = some v₁) :
   ∃ v₂,
-    (Map.mk kvs₂).find? k = some v₂
+    (Map.mk kvs₂).find? k = some v₂ ∧ r (k,v₁) (k,v₂)
   := by
   cases kvs₁ <;> cases kvs₂
   case _ =>
@@ -1462,6 +1477,10 @@ theorem map_find_other_key {α β : Type}
       subst eq
       exists b_value
       simp [Map.find?, List.find?]
+      cases h₂
+      simp at h₄
+      subst h₄
+      assumption
     case false =>
       cases h₂
       rename_i head_prop tail_prop
@@ -1539,6 +1558,34 @@ theorem map_preserves_attrprops₃ {α β : Type}
   apply h₄
   apply h₅
 
+def flip {α β : Type} (r : (Attr × α) → (Attr × β) → Prop) : (Attr × β) → (Attr × α) → Prop :=
+  λ pair₁ pair₂ => r pair₂ pair₁
+
+theorem flip_attr_relation {α β : Type} {r : (Attr × α) → (Attr × β) → Prop}
+  (h : AttributeRelation r) :
+  AttributeRelation (flip r)
+  := by
+  simp [AttributeRelation, flip]
+  intros lhs rhs h'
+  simp [AttributeRelation] at h
+  rw [h]
+  assumption
+
+theorem flip_list_forall {α β : Type} {r : (Attr × α) → (Attr × β) → Prop} {kvs₁ : List (Attr × α)} {kvs₂ : List (Attr × β)}
+  (h : List.Forall₂ r kvs₁ kvs₂) :
+  List.Forall₂ (flip r) kvs₂ kvs₁
+  := by
+  cases h
+  case nil =>
+    constructor
+  case cons head₁ head₂ tail₁ tail₂ prop_head prop_tail =>
+    constructor
+    case _ =>
+      simp [flip, prop_head]
+    case _ =>
+      apply flip_list_forall
+      assumption
+
 
 
 theorem evaluates_to_well_formed_record {attrs : List (Attr × Expr)} {v : Value} {request : Request} {entities : Entities} {env : Environment} {c₁ c₂ : Capabilities} {l₁ : Level}
@@ -1557,7 +1604,6 @@ theorem evaluates_to_well_formed_record {attrs : List (Attr × Expr)} {v : Value
   clear hsound₂
   have hinv := type_of_record_inversion h₃
   replace ⟨_, rty, hinv₁, hinv⟩ := hinv
-
   subst hinv₁
   cases hsound₃
   rename_i attr_map hsound₃ hsound₄ hsound₅
@@ -1570,39 +1616,80 @@ theorem evaluates_to_well_formed_record {attrs : List (Attr × Expr)} {v : Value
     intros k v qty hin_value hin_type
     have evals := record_evaluation attrs attr_map h₅
     replace ⟨vs, evals, evals_sameattrs, eval_map_eq⟩ := evals
-    have well_typed := record_typing attrs (.record (Map.make rty)) h₃
-    replace ⟨tys, well_typed, typed_sameattrs⟩ := well_typed
+    have well_typed := record_typing attrs (Map.make rty) h₃
+    replace ⟨tys, well_typed, typed_sameattrs, ty_map_eq⟩ := well_typed
+    cases h_ty_map : (Map.make rty)
+    rename_i types_canonical
+    rw [ty_map_eq] at h_ty_map
     have exprmap : ∃ m, m = Map.make attrs := by
       exists Map.make attrs
     replace ⟨exprmap, hexprmap⟩ := exprmap
     cases exprmap
     rename_i attrs_canonical
-
-
-
-    sorry
-
-
-
-
-
-
-
-
-
-
-    -- have hstep := record_eval_step₃ attrs attr_map k v h₅ hin_value
-    -- have ⟨e, hstep₁, hstep₂⟩ := hstep
-
-    -- have htyped := record_typing_step attrs ((rty)) k e qty h₃ hin_type hstep₁
-    -- replace ⟨c₂', htyped⟩ := htyped
-    -- apply ih
-    -- apply hstep₁
-    -- apply h₁
-    -- apply h₂
-    -- apply htyped
-    -- apply hstep₂
-    -- assumption
+    cases attr_map
+    rename_i values_canonical
+    have ⟨exprs_evaluate_to_values, expr_values_sameattrs⟩ : List.Forall₂ (EvaluatesToOk request entities) attrs_canonical values_canonical ∧ SameAttrs attrs_canonical values_canonical := by
+      simp [Map.make] at eval_map_eq
+      rw [eval_map_eq]
+      simp [Map.make] at hexprmap
+      rw [hexprmap]
+      refine
+        canonicalize_preserves_attr_relations (EvaluatesToOk request entities) attrs vs evals ?h₂
+          evals_sameattrs
+      exact evalutesToOk_is_AttributeRelation request entities
+    have matching_expr : ∃ e, (Map.mk attrs_canonical).find? k = some e ∧ (flip (EvaluatesToOk request entities)) (k, v) (k, e) := by
+      apply map_find_other_key
+      apply flip_attr_relation
+      apply evalutesToOk_is_AttributeRelation
+      apply flip_list_forall
+      apply exprs_evaluate_to_values
+      apply SameAttrs_com
+      apply expr_values_sameattrs
+      assumption
+    have ⟨e, expr_find, expr_evals⟩ := matching_expr
+    clear matching_expr
+    simp [flip, EvaluatesToOk] at expr_evals
+    have ⟨well_typed_canoncial, attrs_types_canonical_sameattrs⟩ : List.Forall₂ (AttrExprHasAttrType c₁ env l₁) attrs_canonical types_canonical ∧ SameAttrs attrs_canonical types_canonical := by
+      simp [Map.make] at hexprmap
+      rw [hexprmap]
+      simp [Map.make] at h_ty_map
+      rw [← h_ty_map]
+      apply canonicalize_preserves_attr_relations
+      assumption
+      apply attrExprHasAttrType_is_AttributeRelation
+      assumption
+    have matching_expr : ∃ e, (Map.mk attrs_canonical).find? k = some e ∧ (flip (AttrExprHasAttrType c₁ env l₁)) (k, qty) (k, e) := by
+      apply map_find_other_key
+      apply flip_attr_relation
+      apply attrExprHasAttrType_is_AttributeRelation
+      apply flip_list_forall
+      apply well_typed_canoncial
+      apply SameAttrs_com
+      apply attrs_types_canonical_sameattrs
+      rw [← h_ty_map]
+      rw [← ty_map_eq]
+      assumption
+    have ⟨e', type_find, expr_types⟩ := matching_expr
+    clear matching_expr
+    simp [flip, AttrExprHasAttrType] at expr_types
+    have eq : e = e' := by
+      rw [type_find] at expr_find
+      simp at expr_find
+      simp [expr_find]
+    subst eq
+    have ⟨ty', expr_types₁,c', expr_types₂⟩ := expr_types
+    apply ih k e
+    rw [hexprmap] at expr_find
+    apply Map.in_map_in_constructor
+    rw [← hexprmap]
+    assumption
+    assumption
+    assumption
+    rw [expr_types₁]
+    simp [Qualified.getType]
+    apply expr_types₂
+    assumption
+    assumption
   case _ =>
     apply hsound₅
 
